vale/code/arch/x64/X64.Bytes_Semantics.fst
@@ -253,7 +253,6 @@ let update_operand128_flags_same_domains o v s = match o with
         reveal_opaque update_heap32_def;
         let mem = update_heap32 ptr v.lo0 s.mem in
         assert (Set.equal (Map.domain s.mem) (Map.domain mem));
-        admit();
         let mem = update_heap32 (ptr+4) v.lo1 mem in
         assert (Set.equal (Map.domain s.mem) (Map.domain mem));
         let mem = update_heap32 (ptr+8) v.hi2 mem in
@@ -280,3 +279,73 @@ let eval_ins_domains ins s0 =
     else run (check (TS.taint_match_list srcs t s0.TS.memTaint)) s0.TS.state
   in
   eval_ins_bs_domains i s
+
+(* The following lemmas prove that the unspecified heap remains invariant through execution *)
+
+val update_operand_flags_same_unspecified (dst:operand) (v:nat64) (s:state) : Lemma
+  (let s1 = update_operand_preserve_flags' dst v s in
+  forall x. not (Map.contains s1.mem x && Map.contains s.mem x) ==> s1.mem.[x] == s.mem.[x])
+  [SMTPat (update_operand_preserve_flags' dst v s)]
+
+let update_operand_flags_same_unspecified dst v s = match dst with
+  | OMem _ -> reveal_opaque update_heap64_def
+  | _ -> ()
+
+val update_operand_same_unspecified (dst:operand) (ins:ins) (v:nat64) (s:state) : Lemma
+  (let s1 = update_operand' dst ins v s in
+  forall x. not (Map.contains s1.mem x && Map.contains s.mem x) ==> s1.mem.[x] == s.mem.[x])
+  [SMTPat (update_operand' dst ins v s)]
+  
+let update_operand_same_unspecified dst ins v s = update_operand_flags_same_unspecified dst v s
+
+val update_operand128_flags_same_unspecified (o:mov128_op) (v:quad32) (s:state) : Lemma
+  (let s1 = update_mov128_op_preserve_flags' o v s in
+  forall x. not (Map.contains s1.mem x && Map.contains s.mem x) ==> s1.mem.[x] == s.mem.[x])
+  [SMTPat (update_mov128_op_preserve_flags' o v s)]
+
+val update_heap32_same_unspecified (ptr:int) (v:nat32) (h:heap) : Lemma
+  (requires 
+    valid_addr ptr h /\ valid_addr (ptr+1) h /\
+    valid_addr (ptr+2) h /\ valid_addr (ptr+3) h)
+  (ensures (
+    let h1 = update_heap32 ptr v h in
+    (forall x. valid_addr x h <==> valid_addr x h1) /\
+    (forall x. not (Map.contains h1 x && Map.contains h x) ==> h1.[x] == h.[x]))
+  )
+  
+let update_heap32_same_unspecified ptr v h = reveal_opaque update_heap32_def
+
+let update_operand128_flags_same_unspecified o v s = match o with
+  | Mov128Mem m ->
+      let ptr = eval_maddr m s in
+      if not (valid_addr128 ptr s.mem) then ()
+      else
+        // This line is unusued, but needed
+        let s1 = update_mem128 ptr v s in
+        update_heap32_same_unspecified ptr v.lo0 s.mem;
+        let mem = update_heap32 ptr v.lo0 s.mem in
+        update_heap32_same_unspecified (ptr+4) v.lo1 mem;
+        let mem = update_heap32 (ptr+4) v.lo1 mem in
+        update_heap32_same_unspecified (ptr+8) v.hi2 mem;  
+        let mem = update_heap32 (ptr+8) v.hi2 mem in
+        update_heap32_same_unspecified (ptr+12) v.hi3 mem;  
+        let mem = update_heap32 (ptr+12) v.hi3 mem in
+        ()
+  | _ -> ()
+
+val eval_ins_bs_same_unspecified (ins:ins) (s0:state) : Lemma
+  (let Some s1 = eval_code (Ins ins) 0 s0 in
+   forall x. not (Map.contains s1.mem x) ==> s1.mem.[x] == s0.mem.[x])
+
+let eval_ins_bs_same_unspecified ins s0 = ()
+
+let eval_ins_same_unspecified ins s0 =
+  let t = ins.TS.t in
+  let i, dsts, srcs = ins.TS.ops in
+  let s = 
+    if MOVDQU? i then 
+      let MOVDQU dst src, _, _ = ins.TS.ops in
+      run (check (TS.taint_match128 src t s0.TS.memTaint)) s0.TS.state
+    else run (check (TS.taint_match_list srcs t s0.TS.memTaint)) s0.TS.state
+  in
+  eval_ins_bs_same_unspecified i s
